incr/IncrI.v
@@ -1,29 +1,6 @@
 Require Import CRIS.
 Require Import ImpPrelude IncrHeader MemHeader SchHeader.
 
-Module FaaI. Section FaaI.
-  Context {Σ : GRA}.
-
-  Definition scopes : list string := [].
-
-  Definition faa : list val → itree pmodE unit :=
-    λ arg,
-      𝒴;;; '_ : val <- MemHdr.faa arg;;
-      𝒴;;; Ret tt.
-
-  Definition fnsems := [(FaaHdr.faa, (scopes, cfunU faa))].
-
-  Program Definition Mod : PMod.t := {|
-    PMod.scopes := scopes;
-    PMod.fnsems := fnsems;
-    PMod.initial_st := [];
-  |}.
-  Solve All Obligations with prove_scope.
-  Next Obligation. prove_nodup. Qed.
-
-  Definition t : HMod.t := Seal.sealing CRIS (PMod.to_hmod Mod).
-End FaaI. End FaaI.
-
 Module IncrI. Section IncrI.
   Context {Σ : GRA}.
 
@@ -31,7 +8,6 @@ Module IncrI. Section IncrI.
 
   Definition incr : list val → itree pmodE unit :=
     λ arg,
-      𝒴;;; '_ : unit <- ccallU FaaHdr.faa arg;;
       𝒴;;; '_ : unit <- ccallU FaaHdr.faa arg;;
       𝒴;;; Ret tt.
 
