incr/IncrIAproof.v
@@ -1,64 +1,6 @@
 Require Import CRIS.
-Require Import IncrI IncrA SchA MemA SchTactics.
+Require Import IncrI IncrA SchA MemA SchTactics FAA2.
 From iris Require Import frac_auth numbers.
-
-Module FaaIA. Section FaaIA.
-  Context `{!invG α Σ Γ, !subG Γ Σ, !sinvG Σ Γ α β τ}.
-  Context `{!SchAGΣ Σ, !SchAGΓ Γ, !memGΓ Γ}.
-  Context (u_s u_mem : univ_id).
-  Context (spc_s spc_mem spc_user_s : string → option fspec).
-  Context (SchInSpc : spc_incl (SchAS.spc u_s spc_user_s) spc_s).
-
-  Definition Ist : nat → alist key Any.t → alist key Any.t → iProp Σ := λ _ _ _, emp%I.
-
-  Local Definition MemA := (MemA.t u_mem spc_mem).
-  Local Definition FaaA := (FaaA.t u_s spc_s).
-  Local Definition FaaI := (FaaI.t).
-  Local Definition IstFull := (IstProd (IstSB FaaA.(HMod.scopes) Ist) IstEq).
-  Local Definition MA := (FaaA ★ MemA).
-  Local Definition MI := (FaaI ★ MemA).
-
-  Lemma faa_simF : HSim.sim_fun open MA MI IstFull FaaHdr.faa.
-  Proof.
-    init_simF u_s 0.
-    steps_l. iDestruct "ASM" as "[TID [-> ->]]". hss. rename q3 into b, q4 into ofs, q1 into tid.
-    steps_l. steps_r.
-
-    (* tgt yield *)
-    sch_yield_r.
-    iFrame. clear nths st_src st_tgt NODD NODS. iIntros (nths st_s st_t NODS NODD) "IST TID".
-    (* src yield *)
-    sch_yield_l.
-    (* src take pointsto *)
-    steps_l. rename q into v.
-    (* tgt inline - load *)
-    rewrite /MemHdr.faa. inline_r.
-    (* tgt prove preconditions for load *)
-    force_r (b, ofs, Vint v, 1%Qp). forces_r. iFrame. iSplit; first eauto.
-    (* tgt get postconditions from load *)
-    steps_r. iDestruct "GRT" as "[[PT ->] ->]". hss. steps_r.
-    (* tgt inline - store *)
-    inline_r. force_r (b, ofs, Vint (v + 1)). forces_r. iFrame. iSplit; first eauto.
-    (* tgt get postconditions from store *)
-    steps_r. iDestruct "GRT" as "[[PT ->] ->]". hss. steps_r.
-    (* src give pointsto *)
-    force_l. iFrame. steps_l.
-    (* tgt yield *)
-    sch_yield_r.
-    iFrame. clear nths st_s st_t NODD NODS. iIntros (nths st_s st_t NODS NODD) "IST TID".
-    (* tgt terminate *)
-    steps_r.
-    (* src yield & terminate *)
-    sch_yield_l. steps_l. forces_l. iFrame. iSplit; eauto. steps_l. step. iFrame. done.
-  (*FAST*)Qed.
-
-  Lemma sim : HSim.t open MA MI emp%I IstFull.
-  Proof.
-    init_sim.
-    { iIntros "_"; iExists [], [], [], []; eauto. }
-    { eapply faa_simF. }
-  Qed.
-End FaaIA. End FaaIA.
 
 Module IncrIA. Section IncrIA.
   Import IncrAS.
@@ -137,18 +79,6 @@ Module IncrIA. Section IncrIA.
     sch_yield_r. iFrame.
     clear nths st_s st_t NODS NODD. iIntros (nths st_s st_t NODS NODD) "IST".
 
-    steps_r. iDestruct "GRT" as "[TID [-> _]]". hss. steps_r.
-
-    sch_yield_r. iFrame.
-    clear nths st_s st_t NODS NODD. iIntros (nths st_s st_t NODS NODD) "IST TID".
-    (* tgt inline - faa *)
-    inline_r. hss. steps_r. force_r (tid, (b, ofs)). forces_r. iFrame. iSplit; eauto. steps_r. hss.
-    steps_r.
-
-    sch_yield_r.
-    iSplitL "IST"; iFrame.
-    clear nths st_s st_t NODS NODD. iIntros (nths st_s st_t NODS NODD) "IST".
-
     rewrite /IncrAS.incr_inv.
     iInv "INV" as "I" "IA". SL_red.
     clear x. iDestruct "I" as (x) "PT". SL_red. iDestruct "PT" as "[PT CA]".
@@ -162,7 +92,6 @@ Module IncrIA. Section IncrIA.
 
     sch_yield_r. iFrame.
     clear nths st_s st_t NODS NODD. iIntros (nths st_s st_t NODS NODD) "IST".
-
     steps_r. iDestruct "GRT" as "[TID [-> _]]". hss. steps_r.
 
     sch_yield_r. iFrame.
